Arithmetization/ISigmaOne/Metamath/Proof/Theory.lean
@@ -1,0 +1,195 @@
+import Arithmetization.ISigmaOne.Metamath.Formula.Typed
+import Arithmetization.ISigmaOne.Metamath.Proof.Derivation
+
+/-!
+
+# Formalized Theory
+
+-/
+
+noncomputable section
+
+namespace LO.Arith
+
+open FirstOrder FirstOrder.Arith
+
+variable {V : Type*} [Zero V] [One V] [Add V] [Mul V] [LT V] [V ⊧ₘ* 𝐈𝚺₁]
+
+variable {L : Arith.Language V} {pL : LDef} [Arith.Language.Defined L pL]
+
+section FVFree
+
+variable (L)
+
+def Language.IsFVFreeSemiterm (n t : V) : Prop := L.termShift n t = t
+
+def Language.IsFVFree (p : V) : Prop := L.Formula p ∧ L.shift p = p
+
+variable {L}
+
+@[simp] lemma neg_iff : L.IsFVFree (L.neg p) ↔ L.IsFVFree p := by
+  constructor
+  · intro h
+    have hp : L.Formula p := Language.Semiformula.neg_iff.mp h.1
+    have : L.shift (L.neg p) = L.neg p := h.2
+    simp [shift_neg hp, neg_inj_iff hp.shift hp] at this
+    exact ⟨hp, this⟩
+  · intro h; exact ⟨by simp [h.1], by rw [shift_neg h.1, h.2]⟩
+
+
+end FVFree
+
+section theory
+
+variable (L)
+
+structure _root_.LO.FirstOrder.Arith.LDef.TDef (pL : LDef) where
+  ch : HSemisentence ℒₒᵣ 1 𝚺₁
+
+protected structure Language.Theory where
+  set : Set V
+  set_fvFree : ∀ p ∈ set, L.IsFVFree p
+
+instance : Membership V L.Theory := ⟨fun x T ↦ x ∈ T.set⟩
+
+variable {L}
+
+namespace Language.Theory
+
+protected class Defined (T : L.Theory) (pT : outParam pL.TDef) where
+  defined : 𝚺₁-Predicate (· ∈ T.set) via pT.ch
+
+variable (T : L.Theory) {pT : pL.TDef} [T.Defined pT]
+
+instance mem_defined : 𝚺₁-Predicate (· ∈ T) via pT.ch := Defined.defined
+
+instance mem_definable : 𝚺₁-Predicate (· ∈ T) := Defined.defined.to_definable
+
+variable {T}
+
+lemma fvFree_neg_of_mem {p} (hp : p ∈ T) : L.IsFVFree (L.neg p) := by simpa using T.set_fvFree p hp
+
+lemma fvFree_of_neg_mem {p} (hp : L.neg p ∈ T) : L.IsFVFree p := by simpa using T.set_fvFree _ hp
+
+end Language.Theory
+
+end theory
+
+section derivableWithTheory
+
+def Language.Theory.Derivable (T : L.Theory) (s : V) : Prop :=
+  ∃ antecedents : V, (∀ p ∈ antecedents, L.neg p ∈ T) ∧ L.Derivable (antecedents ∪ s)
+
+def Language.Theory.Provable (T : L.Theory) (p : V) : Prop := T.Derivable {p}
+
+section
+
+def _root_.LO.FirstOrder.Arith.LDef.TDef.derivableDef {pL : LDef} (pT : pL.TDef) : 𝚺₁-Semisentence 1 := .mkSigma
+  “s | ∃ a, (∀ p ∈' a, ∃ np, !pL.negDef np p ∧ !pT.ch np) ∧ ∃ uni, !unionDef uni a s ∧ !pL.derivableDef uni” (by simp)
+
+variable (T : L.Theory) {pT : pL.TDef} [T.Defined pT]
+
+protected lemma Language.Theory.derivable_defined : 𝚺₁-Predicate T.Derivable via pT.derivableDef := by
+  intro v; simp [LDef.TDef.derivableDef, (neg_defined L).df.iff,
+    (T.mem_defined).df.iff, (derivable_defined L).df.iff, Language.Theory.Derivable]
+
+instance Language.Theory.derivable_definable : 𝚺₁-Predicate T.Derivable := Defined.to_definable _ T.derivable_defined
+
+/-- instance for definability tactic-/
+@[simp] instance Language.Theory.derivable_definable' : (𝚺, 0 + 1)-Predicate T.Derivable := T.derivable_definable
+
+def _root_.LO.FirstOrder.Arith.LDef.TDef.prv {pL : LDef} (pT : pL.TDef) : 𝚺₁-Semisentence 1 := .mkSigma
+  “p | ∃ s, !insertDef s p 0 ∧ !pT.derivableDef s” (by simp)
+
+protected lemma Language.Theory.provable_defined : 𝚺₁-Predicate T.Provable via pT.prv := by
+  intro v; simp [LDef.TDef.prv, (T.derivable_defined).df.iff, Language.Theory.Provable, singleton_eq_insert, emptyset_def]
+
+instance Language.Theory.provable_definable : 𝚺₁-Predicate T.Provable := Defined.to_definable _ T.provable_defined
+
+/-- instance for definability tactic-/
+@[simp] instance Language.Theory.provable_definable' : (𝚺, 0 + 1)-Predicate T.Provable := T.provable_definable
+
+end
+
+namespace Language.Theory.Derivable
+
+variable {T : L.Theory} {pT : pL.TDef} [T.Defined pT]
+
+lemma by_axm (hs : L.FormulaSet s) {p} (hpT : p ∈ T) (hp : p ∈ s) : T.Derivable s :=
+  ⟨{L.neg p}, by simp [neg_neg (hs p hp), hpT], Language.Derivable.em (p := p) (by simp [hs, hs p hp]) (by simp [hp]) (by simp)⟩
+
+lemma verum (hs : L.FormulaSet s) (h : ^⊤ ∈ s) : T.Derivable s :=
+  ⟨∅, by simp, Language.Derivable.verum (by simp [hs]) (by simp [h])⟩
+
+lemma em (hs : L.FormulaSet s) (p : V) (h : p ∈ s) (hn : L.neg p ∈ s) : T.Derivable s :=
+  ⟨∅, by simp, Language.Derivable.em (p := p) (by simpa) (by simp [h]) (by simp [hn])⟩
+
+lemma and {p q : V} (dp : T.Derivable (insert p s)) (dq : T.Derivable (insert q s)) : T.Derivable (insert (p ^⋏ q) s) := by
+  rcases dp with ⟨Γ, hΓ, dp⟩
+  rcases dq with ⟨Δ, hΔ, dq⟩
+  exact ⟨Γ ∪ Δ, by intro x hx; rcases mem_cup_iff.mp hx with (hx | hx); { exact hΓ x hx }; { exact hΔ x hx },
+    Language.Derivable.and_m (p := p) (q := q) (by simp)
+      (Language.Derivable.wk (by simp [by simpa using dp.formulaSet, by simpa using dq.formulaSet])
+        (by intro x; simp; tauto) dp)
+      (Language.Derivable.wk (by simp [by simpa using dp.formulaSet, by simpa using dq.formulaSet])
+        (by intro x; simp; tauto) dq)⟩
+
+lemma or {p q : V} (dpq : T.Derivable (insert p (insert q s))) : T.Derivable (insert (p ^⋎ q) s) := by
+  rcases dpq with ⟨Γ, hΓ, d⟩
+  exact ⟨Γ, hΓ, Language.Derivable.or_m (p := p) (q := q) (by simp)
+    (d.wk (by simp [by simpa using d.formulaSet]) <| by intro x; simp; tauto)⟩
+
+lemma all {p : V} (hp : L.Semiformula 1 p) (dp : T.Derivable (insert (L.free p) (L.setShift s))) : T.Derivable (insert (^∀ p) s) := by
+  rcases dp with ⟨Γ, hΓ, d⟩
+  have hs : L.setShift Γ = Γ := mem_ext <| by
+    simp only [mem_setShift_iff]; intro x
+    constructor
+    · rintro ⟨x, hx, rfl⟩; simpa [fvFree_of_neg_mem (hΓ x hx) |>.2] using hx
+    · intro hx; exact ⟨x, hx, by simp [fvFree_of_neg_mem (hΓ x hx) |>.2]⟩
+  exact ⟨Γ, hΓ,
+    Language.Derivable.all_m (p := p) (by simp)
+      (Language.Derivable.wk (by simp [by simpa using d.formulaSet, hp])
+        (by intro x; simp [hs]; tauto) d)⟩
+
+lemma ex {p t : V} (hp : L.Semiformula 1 p) (ht : L.Term t)
+    (dp : T.Derivable (insert (L.substs₁ t p) s)) : T.Derivable (insert (^∃ p) s) := by
+  rcases dp with ⟨Γ, hΓ, d⟩
+  exact ⟨Γ, hΓ, Language.Derivable.ex_m (p := p) (by simp) ht
+    (Language.Derivable.wk (by simp [by simpa using d.formulaSet, hp]) (by intro x; simp; tauto) d)⟩
+
+lemma wk {s s' : V} (h : L.FormulaSet s) (hs : s' ⊆ s) (d : T.Derivable s') : T.Derivable s := by
+  rcases d with ⟨Γ, hΓ, d⟩
+  exact ⟨Γ, hΓ, Language.Derivable.wk (by simp [by simpa using d.formulaSet, h]) (by intro x; simp; tauto) d⟩
+
+lemma cut {s : V} (p : V) (d : T.Derivable (insert p s)) (dn : T.Derivable (insert (L.neg p) s)) : T.Derivable s := by
+  rcases d with ⟨Γ, hΓ, d⟩; rcases dn with ⟨Δ, hΔ, b⟩
+  exact ⟨Γ ∪ Δ, fun p hp ↦ by rcases mem_cup_iff.mp hp with (h | h); { exact hΓ p h }; { exact hΔ p h },
+    Language.Derivable.cut p
+      (Language.Derivable.wk
+        (by simp [by simpa using d.formulaSet, by simpa using b.formulaSet]) (by intro x; simp; tauto) d)
+      (Language.Derivable.wk
+        (by simp [by simpa using d.formulaSet, by simpa using b.formulaSet]) (by intro x; simp; tauto) b)⟩
+
+/-- Crucial inducion for formalized $\Sigma_1$-completeness. -/
+lemma conj (ps : V) {s} (hs : L.FormulaSet s)
+    (ds : ∀ i < len ps, T.Derivable (insert ps.[i] s)) : T.Derivable (insert (^⋀ ps) s) := by
+  have : ∀ k ≤ len ps, T.Derivable (insert (^⋀ (takeLast ps k)) s) := by
+    intro k hk
+    induction k using induction_iSigmaOne
+    · definability
+    case zero => simpa using verum (by simp [hs]) (by simp)
+    case succ k ih =>
+      simp [takeLast_succ_of_lt (succ_le_iff_lt.mp hk)]
+      have ih : T.Derivable (insert (^⋀ takeLast ps k) s) := ih (le_trans le_self_add hk)
+      have : T.Derivable (insert ps.[len ps - (k + 1)] s) := ds (len ps - (k + 1)) ((tsub_lt_iff_left hk).mpr (by simp))
+      exact this.and ih
+  simpa using this (len ps) (by rfl)
+
+end Language.Theory.Derivable
+
+
+end derivableWithTheory
+
+
+
+end LO.Arith
